# 1.13

$$ \phi\frac{d\phi}{dx} = \frac{1}{2}\frac{d(\phi^2)}{dx} $$

より，以下の2種類の離散化をおこなう．

$$ \frac{\phi_{n+1} - 2\phi_n + \phi_{n-1}}{\Delta x^2} = K^1(\phi)_n $$

$$ K^1(\phi)_n = \phi_n\frac{\phi_{n+1} - \phi_{n-1}}{2\Delta x} $$

$$ \frac{\phi_{n+1} - 2\phi_n + \phi_{n-1}}{\Delta x^2} = K^2(\phi)_n $$

$$ K^2(\phi)_n = \frac{\phi_{n+1}^2 - \phi_{n-1}^2}{4\Delta x} $$

これを繰り返しによって解くと，回の反復後に

$$ \phi^1 = \left[ \begin{array}{c}  \end{array} \right] $$

$$ \phi^2 = \left[ \begin{array}{c}  \end{array} \right] $$

を得る．
